Up to date

Vector.v
@@ -1,9 +1,49 @@
 Require Import Ring.
 Require Import Coq.Array.PArray.
-
+Require Import Coq.Numbers.Cyclic.Int63.Int63.
 
 Print Ring.
+(*
+Inductive Vector {A : Type} : A -> Int63.int -> Type :=
+| Hello (ar : array A) : (array A) -> Vector A (length ar).
+*)                               
 
-Inductive Vector {A : Type} : nat -> Type :=
-| Hello : Vector 3.
-                                 
+Inductive NatHolder : Type :=
+| Hello : NatHolder
+| Hold (x : nat) : NatHolder.
+
+Inductive Vector (A : Type) : int -> Type :=
+| vect (arr : array A) : Vector A (length arr).
+
+Definition example_vector : Vector nat 3 :=
+  vect _ (make 3 3).
+
+Print example_vector.
+
+Definition test : nat :=
+  match example_vector with
+  | vect _ ar => get ar 0
+  end.
+
+Theorem t1 :  test = 3.
+Proof.
+  unfold test.
+  unfold example_vector.
+  unfold make.
+  unfold get.
+  reflexivity.
+Qed.
+
+
+Definition example_vector2 : Vector nat 3 :=
+  vect _ ([| 1 ; 2 ; 3 | 4 : nat |]).
+
+Definition length {A : Type} {n : int} : Vector A n -> int :=
+  fun v => n.
+
+Theorem t2 : (length example_vector) = 3.
+
+Show (length example_vector2).
+
+Search array.
+Print array.
